{"nbformat":4,"nbformat_minor":0,"metadata":{"colab":{"provenance":[],"authorship_tag":"ABX9TyPQe8uLqHeJH27/0HIZ04a6"},"kernelspec":{"name":"python3","display_name":"Python 3"},"language_info":{"name":"python"}},"cells":[{"cell_type":"markdown","source":["###An Introduction to Penrose-Pseudo Inverse"],"metadata":{"id":"6p9IlrVDtlUT"}},{"cell_type":"markdown","source":["The Penrose-Pseudo Inverse $A^{+}$ of a matrix $A$ is a type of matrix that is useful in situations where the inverse matrix does not exist.\n","\n","$A^{-1}$ exists if $det(A) \\neq 0.$\n","If $A^{-1}$ exists, $A^{+} = A^{-1}$.\n","\n","The Penrose-Pseudo Inverse is possible to be calculated in most matrixes and there are a number of methods to calculate it. The most common is Singular Value Decomposition which is already implemented in Python with np.linalg.pinv(). "],"metadata":{"id":"upB0rTitVahZ"}},{"cell_type":"code","source":["import numpy as np\n","\n","\n","A = np.array([[3, 2] , [6, 4]])\n","\n","print(\"Matrix A:\")\n","print(A)\n","\n","#Ainv = np.linalg.inv(A); #will compute error, since this matrix's det = 0.\n","#(numpy.linalg.LinAlgError: Singular matrix.) \n","\n","Apinv = np.linalg.pinv(A); #calculate pseudo-inverse\n","\n","print(\"Matrix A pseudo-inverse (G):\")\n","print(Apinv)"],"metadata":{"id":"Av8mVh98h4rg"},"execution_count":null,"outputs":[]},{"cell_type":"markdown","source":["Another popular way to calculate it is by as defined by Moore-Penrose:\n","\n","$A^{+} = (A^TA)^{-1}A^T$\n","\n","\n","Moore-Penrose Pseudo-Inverses have 4 major properties:\n","\n","1. $AGA = A$"],"metadata":{"id":"HSxglSm8iBVZ"}},{"cell_type":"code","source":["print(\"\\nTest of theorem 1 - AGA = A\")\n","print(np.dot(np.dot(A, Apinv), A))"],"metadata":{"id":"RltJ_2rkiylX"},"execution_count":null,"outputs":[]},{"cell_type":"markdown","source":["2. $GAG = G$"],"metadata":{"id":"veJrwDLUi1mH"}},{"cell_type":"code","source":["print(\"\\nTest of theorem 2 - GAG = G\")\n","print(np.dot(np.dot(Apinv, A), Apinv))"],"metadata":{"id":"1PNWcYLmi8lk"},"execution_count":null,"outputs":[]},{"cell_type":"markdown","source":["3. $(AG)^{T} = AG$"],"metadata":{"id":"9qUSFuGAi_3Y"}},{"cell_type":"code","source":["print(\"\\nTest of theorem 3 - AG^T = AG\")\n","print(\"\\nAG =\")\n","AG = np.dot(A, Apinv)\n","print(AG)\n","print(\"\\nAG^T =\")\n","AGt = AG.transpose()\n","print(AGt)"],"metadata":{"id":"2z-OuYKQjJZM"},"execution_count":null,"outputs":[]},{"cell_type":"markdown","source":["4. $(GA)^T = GA$"],"metadata":{"id":"VlLGUeZWjMIW"}},{"cell_type":"code","source":["print(\"\\nTest of theorem 4 - GAT = GA\")\n","GA = np.dot(Apinv, A)\n","\n","print(\"\\n GA = \")\n","print(GA)\n","\n","GAt = GA.transpose()\n","print(\"GA^T =\")\n","print(GAt)"],"metadata":{"id":"Kvg_N4nljRyn"},"execution_count":null,"outputs":[]}]}